basic.v
@@ -6,6 +6,7 @@ Set Implicit Arguments.
 Ltac split_refl eq_dec a := let H:= fresh in destruct (eq_dec a a) as [H|bad]; [clear H|contradict bad]; auto.
 Ltac split_refl2 eq_dec a a' := let H:= fresh in
                                 destruct (eq_dec a a') as [bad|H]; [contradict bad|clear H]; auto.
+Ltac unf f := unfold f; fold f.
 Ltac bad_eq := match goal with [Hbad : ?a <> ?a |- _] => contradict Hbad; auto end.
 Ltac inject_pair := match goal with [H: (?a, ?b) = (?c, ?d) |- _] => injection H; intros; subst end.
 Ltac inverts H := inversion H; subst.
